s/SecurityGateway/PolEnforcePoint/

thy/Network_Security_Policy_Verification/Examples/Example_Forte14.thy
@@ -57,9 +57,9 @@ definition DomainHierarchy_m::"(string SecurityInvariant)" where
               Department ''crew'' []
             ])" by eval
 
-definition SecurityGateway_m::"(string SecurityInvariant)" where
-  "SecurityGateway_m \<equiv> new_configured_list_SecurityInvariant SINVAR_LIB_SecurityGatewayExtended \<lparr> 
-          node_properties = [''IFEsrv'' \<mapsto> SINVAR_SecGwExt.SecurityGatewayIN,
+definition PolEnforcePoint_m::"(string SecurityInvariant)" where
+  "PolEnforcePoint_m \<equiv> new_configured_list_SecurityInvariant SINVAR_LIB_PolEnforcePointExtended \<lparr> 
+          node_properties = [''IFEsrv'' \<mapsto> SINVAR_SecGwExt.PolEnforcePointIN,
                              ''IFE1'' \<mapsto> SINVAR_SecGwExt.DomainMember,
                              ''IFE2'' \<mapsto> SINVAR_SecGwExt.DomainMember]
           \<rparr> ''IFEsrc mediates access of its thin clients''"
@@ -81,7 +81,7 @@ definition BLP_m::"(string SecurityInvariant)" where
                              ''IFEsrv'' \<mapsto> \<lparr> security_level = 0, trusted = True \<rparr>]
           \<rparr> ''Confidential data''"
 
-definition "security_invariants = [ DomainHierarchy_m, SecurityGateway_m, BLP_m]"
+definition "security_invariants = [ DomainHierarchy_m, PolEnforcePoint_m, BLP_m]"
 
 lemma "all_security_requirements_fulfilled security_invariants policy" by eval
 
